Core of correctness proof of Kildall algorithm
Currently assumes that all reachable nodes are reachable, which breaks
the final proof.

src/coq/Analysis/Kildall.v
@@ -28,98 +28,933 @@
 
 *)
 
-Require Import Equalities Orders.
-Require Import FMaps.
-
+From Coq Require Import List Equalities Orders Classes.RelationClasses Program.Equality.
 
 From Vellvm.Analysis Require Import
      Iteration
      Lattice.
 
+From MathClasses Require interfaces.orders interfaces.abstract_algebra orders.lattices.
+Import (hints) interfaces.canonical_names interfaces.orders interfaces.abstract_algebra orders.lattices.
+(* Print Instances abstract_algebra *)
 
-Module FMapProps (E:UsualDecidableType) (M:FMapInterface.WSfun E).
+Module Framework.
+  From MathClasses Require Import canonical_names.
 
-  #[local] Notation K := M.key.
+  Class Framework `{Ae: Equiv A} (Ale: Le A) `{Meet A} `{Join A} :=
+    make   {
+        (* The lattice L. *)
+        lattice:: orders.LatticeOrder Ale;
+        top: A;
 
-  Section FMapProps.
+        (* A set of transfer functions, indexed by I.  *)
+        I: Type;
+        fs: I -> A -> A;
+        fs_proper:: Proper ((@eq I) ==> canonical_names.equiv ==> canonical_names.equiv) fs;
+      }.
+End Framework.
+Export Framework(Framework).
+Export (hints) Framework.
 
-  Variable V : Type.
+Module Instance.
+  From MathClasses Require Import canonical_names.
+  Import Framework.
 
-  Definition find_default (m:M.t V) (k:K) (d:V) : V :=
-    match M.find k m with
-      | None => d
-      | Some m => m
-    end.
+  Class Instance `{Ae: Equiv A} `{Ale: Le A} `{Meet A} `{Join A} (framework: Framework Ale) :=
+    make {
+        Node: Type;
+        root: Node;
+        (* Could by any foldable. *)
+        successors: Node -> list Node;
+        label: Node -> framework.(I);
+      }.
 
-  Lemma find_default_neq : forall  m n1 n2 l d,
-    n1 <> n2 ->
-    find_default (M.add n1 l m) n2 d = find_default m n2 d.
+  Definition transfer `{instance: Instance} (n: Node): A -> A := Framework.fs (label n).
+
+  Add Parametric Morphism `{instance: Instance} (n: Node): (transfer n)
+      with signature canonical_names.equiv ==> canonical_names.equiv as transfer_morphism.
   Proof.
-    intros. unfold find_default.
-    destruct (M.find n2 (M.add _ _ _)) eqn:Heq1, (M.find n2 m) eqn:Heq2.
-    apply M.find_2 in Heq1. apply M.add_3 in Heq1; auto. apply M.find_1 in Heq1.
-      rewrite Heq2 in Heq1. injection Heq1. auto.
-    apply M.find_2 in Heq1. apply M.add_3 in Heq1; auto. apply M.find_1 in Heq1.
-      rewrite Heq2 in Heq1. discriminate Heq1.
-    apply M.find_2 in Heq2. eapply M.add_2 in Heq2; eauto. apply M.find_1 in Heq2.
-      rewrite Heq2 in Heq1. discriminate Heq1.
-    trivial.
+    intros x y x_Eqv_y. (* unfold transfer. rewrite -> x_Eqv_y. *)
+    apply framework.(fs_proper).
+    - reflexivity.
+    - assumption.
   Qed.
 
-  Lemma find_default_eq : forall m n1 n2 l d,
-    n1 = n2 ->
-    find_default (M.add n1 l m) n2 d = l.
+End Instance.
+Export Instance(Instance).
+Export (hints) Instance.
+Print Instances Proper.
+
+Module Solver.
+  Section Global.
+    From stdpp Require base decidable countable gmap.
+    Import (notations) base. Import base(dom).
+
+    (* For now, let's assume N (the set of graph nodes) countable.
+         We only actually need that the set of reachable Ns is countable.
+         A is the analysis domain, aka the framework's lattice.
+     *)
+    (* BUG: Why is A explicit? Why do we have to resort to this weird named parameter thing?
+         https://github.com/coq/coq/issues/10272
+     *)
+    Context {A: Type} `{instance: (Instance A (framework := framework))} `{Countable_N: countable.Countable Instance.Node}.
+    Notation N := (Instance.Node).
+    Notation Map := (gmap.gmap N A).
+
+    Notation "x '?!' y" := (match x !! y with | None => ⊤ | Some v => v end)
+                             (at level 1).
+
+    Instance top_le: base.Top A := Framework.top (A := A).
+    Instance sqsubseteq_le: base.SqSubsetEq A := canonical_names.le (A := A).
+    Instance meet_meet: base.Meet A := canonical_names.meet (A := A).
+
+    Class Analysis :=
+      make {
+          fixpoint: Map -> option Map;
+          fixpoint_solution: forall (init result: Map) (n s: N),
+            fixpoint init = Some result -> n ∈ dom(init) -> s ∈ (Instance.successors n) -> (result ?! s) ⊑ Instance.transfer n (result ?! n);
+          fixpoint_invariant: forall (P: N -> A -> Prop) (init result: Map),
+            fixpoint init = Some result ->
+            (forall n, P n (init ?! n)) ->
+            (forall (p n: N) (pApprox nApprox: A), P p pApprox -> P n nApprox ->
+                                              n ∈ (Instance.successors p) ->
+                                              P n (nApprox ⊓ (Instance.transfer p pApprox))) ->
+            forall (n: N), P n (result ?! n);
+        }.
+
+    Section Lemmas.
+      Context `{analysis: Analysis} (init result: Map) (Def_result: fixpoint init = Some result).
+
+      Lemma fixpoint_entry: forall (n: N), (result ?! n) ⊑ (init ?! n).
+      Proof.
+        intros n.
+        apply fixpoint_invariant with (init := init); [assumption| |]; clear n.
+        - intros n; generalize (init ?! n); clear n. intros l.
+          reflexivity.
+        - intros p n pApprox nApprox IH_p IH_n Successor_n.
+          (* For some reason, apply doesn't work...  *)
+          unfold "⊓" in *.
+          apply (lattices.meet_le_compat_r _ _ _ IH_n).
+      Qed.
+
+    End Lemmas.
+  End Global.
+End Solver.
+
+Module Kildall.
+  From stdpp Require base option countable fin_maps gmap.
+  Import (notations, hints) base. Import base(dom).
+
+  Section Global.
+    Context {A: Type} `{instance: (Instance A (Ae := Ae) (framework := framework))} `{Countable_N: countable.Countable Instance.Node} `{base.RelDecision _ _ (@canonical_names.equiv A Ae)}.
+    Notation N := (Instance.Node).
+    Notation Map := (gmap.gmap N A).
+
+    Record State := mkst { in_flow_map: Map; work: list N }.
+
+    (* Instance top_le: base.Top A := Framework.top (A := A). *)
+    (* Instance default_A: base.Inhabited A := base.populate (Framework.top (A := A)). *)
+    Instance sqsubseteq_le `{canonical_names.Le T}: base.SqSubsetEq T := canonical_names.le (A := T).
+    Instance meet_meet `{canonical_names.Meet T}: base.Meet T := canonical_names.meet (A := T).
+    Instance equiv `{canonical_names.Equiv T}: base.Equiv T := canonical_names.equiv (A := T).
+
+    Definition lookup (m: Map) (n: N) := option.from_option id Framework.top (m !! n).
+    Infix "?!" := lookup (at level 20).
+    Notation "'(' x '?!)'" := (fun (y: N) => (x: Map) ?! y) (at level 0).
+
+    Definition andsb (P Q: Prop) `{base.Decision P} `{base.Decision Q}: {P /\ Q} + {~P \/ ~Q}.
+      destruct (base.decide P).
+      - destruct (base.decide Q).
+        + left; split; assumption.
+        + right. right. assumption.
+      - right. left. assumption.
+    Qed.
+
+    Definition orsb (P Q: Prop) `{base.Decision P} `{base.Decision Q}: {P \/ Q} + {~P /\ ~Q}.
+      destruct (base.decide P).
+      - left. left. assumption.
+      - destruct (base.decide Q).
+        + left. right. assumption.
+        + right. split; assumption.
+    Qed.
+
+    Definition negsb (P: Prop) `{base.Decision P}: {~P} + {P}.
+      destruct (base.decide P).
+      - right. assumption.
+      - left. assumption.
+    Qed.
+
+    Instance and_dec `{base.Decision P} `{base.Decision Q}: base.Decision (P /\ Q).
+    Proof.
+      unfold base.Decision.
+      destruct (base.decide P).
+      - destruct (base.decide Q).
+        + left. split; assumption.
+        + right. rewrite -> decidable.not_and_l. right. assumption.
+      - right. rewrite -> decidable.not_and_l. left. assumption.
+    Qed.
+
+    (* Instance or_dec `{base.Decision P} `{base.Decision Q}: base.Decision (P \/ Q). *)
+    (* Proof. *)
+    (*   unfold base.Decision. *)
+    (*   destruct (base.decide P). *)
+    (*   - left. left. assumption. *)
+    (*   - destruct (base.decide Q). *)
+    (*     + left. right. assumption. *)
+    (*     + right. rewrite -> decidable.not_and_l.  *)
+    (* Qed. *)
+
+
+    Lemma insert_lookup: forall (m: Map) n v, (<[ n := v ]> m) ?! n = v.
+    Proof. intros. unfold lookup,base.insert,fin_maps.map_insert. rewrite -> fin_maps.lookup_partial_alter. reflexivity. Qed.
+
+    Lemma insert_lookup_ne: forall (m: Map) n n' v, n' <> n -> (<[ n' := v ]> m) ?! n = m ?! n.
+    Proof. intros. unfold lookup,base.insert,fin_maps.map_insert. rewrite -> fin_maps.lookup_partial_alter_ne by assumption. reflexivity. Qed.
+
+    Definition in_flow (state: State) (n: N): A := state.(in_flow_map) ?! n.
+    Definition out_flow (state: State) (n: N): A := Instance.transfer n (in_flow state n).
+
+    Arguments in_flow !state /.
+    Arguments out_flow !state /.
+
+    (* Allows using the pointwise lattice on map lookup.
+       This means that one can write
+            (m ?!) ⊑ (n ?!)
+       as a shothand for
+            forall x, (m ?! x) ⊑ (n ?! x)
+     *)
+    Import (hints) Lattices.Pointwise.
+    Instance state_lattice: Lattices.Pointwise.Pointwise N A := {}.
+
+    (* Setoid are really useful (who knew?); let's expose their instances. *)
+    Local Instance setoid `{orders.PartialOrder T}: abstract_algebra.Setoid T.
+    Proof. apply orders.po_setoid. Qed.
+
+    Local Instance meetsemilattice `{orders.MeetSemiLatticeOrder T}: abstract_algebra.MeetSemiLattice T := orders.lattices.meet_sl_order_meet_sl.
+
+    Instance state_equiv: canonical_names.Equiv State := fun s0 s1 => (in_flow s0 ≡ in_flow s1) /\ s0.(work) = s1.(work).
+
+    Instance state_equiv_equiv: Equivalence (@canonical_names.equiv _ state_equiv).
+    Proof.
+      constructor.
+      - intros []. split; reflexivity.
+      - intros [] []. split; symmetry; firstorder.
+      - intros [] [] [] [] []. split; etransitivity; eassumption.
+    Qed.
+
+    Add Morphism in_flow
+        with signature (≡) ==> (=) ==> (≡) as in_flow_morph.
+    Proof. intros [x ?] [y ?] [x_Equiv_y ?]. apply x_Equiv_y. Qed.
+
+    Add Morphism out_flow
+        with signature (≡) ==> (=) ==> (≡) as out_flow_morph.
+    Proof.
+      intros x y x_Equiv_y n. unfold out_flow.
+      apply Instance.transfer_morphism.
+      apply in_flow_morph.
+      - assumption.
+      - reflexivity.
+    Qed.
+
+    Section Implementation.
+      (* Propagate the output of an update to the node n. *)
+      Definition propagate_to (out: A) (s: State) (n: N) : State :=
+        let oldl := in_flow s n in
+        let newl := oldl ⊓ out in
+        if base.decide (oldl ≡ newl /\ n ∈ dom(s.(in_flow_map)))
+        then s else mkst (<[ n := newl  ]>s.(in_flow_map)) (n :: s.(work)).
+
+      Definition step (state: State): Map + State :=
+        match state.(work) with
+        | nil => inl state.(in_flow_map)
+        | n :: rem =>
+            inr (fold_left (propagate_to (out_flow state n))
+                   (Instance.successors n) (mkst state.(in_flow_map) rem))
+        end.
+
+      Definition make_init_state (inits: Map): State :=
+        mkst inits (base.elements (dom(inits))).
+
+      Definition fixpoint (inits: Map): option Map := Iter.iterate step (make_init_state inits).
+    End Implementation.
+
+    Notation "x '~>' y" := (y ∈ (Instance.successors x)) (at level 70, no associativity).
+    Notation "x '~/>' y" := (y ∉ (Instance.successors x)) (at level 70, no associativity).
+
+    Instance decide_succ: base.RelDecision (fun x y => x ~> y).
+    Proof. intros x y. apply (@list.elem_of_list_dec N _ y (Instance.successors x)). Qed.
+
+    Section Invariants.
+
+      Local Definition InitCondition (init: Map) (state: State): Prop :=
+        in_flow state ⊑ (init ?!).
+
+      Local Definition undefined (state: State) (n: N): Prop :=
+        n ∈ state.(work) \/ n ∉ dom(state.(in_flow_map)).
+
+      Local Definition SuccCondition (n: N) (state: State): Prop :=
+        forall p, p ~> n -> (undefined state p \/ in_flow state n ⊑ out_flow state p).
+      Local Tactic Notation "in_work" := left; left.
+      Local Tactic Notation "ignored" := left; right.
+      Local Tactic Notation "satisfies_equation" := right.
+
+      Local Definition Conditions (init: Map) (state: State): Prop :=
+        InitCondition init state /\ forall n, SuccCondition n state.
+
+      Lemma SuccCond_non_pred_weakening: forall n map work w,
+          SuccCondition n (mkst map (w :: work)) ->
+          w ~/> n ->
+          SuccCondition n (mkst map work).
+      Proof.
+        intros n map work w SuccCond w_NotPred_n.
+        intros p p_Pred_n. specialize (SuccCond _ p_Pred_n) as [[Work_p|Ignored_p]|FlowEq_n_w].
+        - cbn in Work_p. rewrite -> list.elem_of_cons in Work_p.
+          destruct Work_p as [?|?].
+          + subst. contradiction.
+          + in_work. assumption.
+        - ignored. assumption.
+        - right.
+          unfold out_flow,in_flow in *. cbn in *.
+          assumption.
+      Qed.
+
+      Lemma SuccCond_strengthening: forall map work w,
+          (forall n, SuccCondition n (mkst map (w :: work))) ->
+          (forall s, w ~> s -> map ?! s ⊑ Instance.transfer w (map ?! w)) ->
+          (forall n, SuccCondition n (mkst map work)).
+      Proof.
+        intros map work w SuccCond Flow_w.
+        intros n. specialize (SuccCond n).
+        destruct (base.decide (w ~> n)) as [w_Pred_n | w_NotPred_n].
+        - intros p p_Pred_n.
+          specialize (SuccCond _ p_Pred_n) as [[Work_p|Ignored_p]|Flow_n_p].
+          + cbn in Work_p. rewrite -> list.elem_of_cons in Work_p.
+            destruct Work_p as [?|?].
+            * subst. satisfies_equation. apply Flow_w. assumption.
+            * in_work. assumption.
+          + ignored. assumption.
+          + satisfies_equation. apply Flow_n_p.
+        - apply SuccCond_non_pred_weakening with (1 := SuccCond) (2 := w_NotPred_n).
+      Qed.
+
+      Local Ltac destruct_propagation_impl H1 H2 H3 :=
+        (lazymatch goal with
+         | [|- context[ propagate_to ?out ?state ?w  ] ] =>
+             unfold propagate_to;
+             destruct (base.decide (in_flow state w ≡ in_flow state w ⊓ out /\ w ∈ dom(in_flow_map state)))
+                      as [[H1 H2] | H3%decidable.not_and_l]
+         end).
+      Tactic Notation "destruct_propagation" :=
+        (let H1 := fresh in let H2 := fresh in let H3 := fresh in
+          destruct_propagation_impl H1 H2 H3).
+      Tactic Notation "destruct_propagation" "as" simple_intropattern(H1) simple_intropattern(H2) simple_intropattern(H3) := (destruct_propagation_impl H1 H2 H3).
+
+      Lemma propagation_smaller: forall out state w,
+          (in_flow (propagate_to out state w)) ⊑ (in_flow state).
+      Proof.
+        intros out state w n.
+        destruct_propagation.
+        - reflexivity.
+        - unfold in_flow, "⊓". cbn.
+          destruct (base.decide (w = n)) as [?|?]; subst.
+          + rewrite -> insert_lookup.
+            apply orders.meet_lb_l.
+          + rewrite -> insert_lookup_ne by assumption.
+            reflexivity.
+      Qed.
+
+      Lemma propagation_equ: forall out state w,
+          w ∈ (propagate_to out state w).(work) \/
+            in_flow (propagate_to out state w) w ≡ in_flow state w.
+      Proof.
+        intros out state w.
+        destruct_propagation.
+        - right. reflexivity.
+        - left. apply base.elem_of_list_here.
+      Qed.
+
+      Lemma propagation_lookup_eq: forall out state w,
+          in_flow (propagate_to out state w) w ≡ in_flow state w ⊓ out.
+      Proof.
+        intros out state w.
+        destruct_propagation.
+        - assumption.
+        - unfold in_flow. cbn. rewrite -> insert_lookup. reflexivity.
+      Qed.
+
+      Lemma propagation_lookup_ne: forall out state w n,
+          w <> n -> in_flow (propagate_to out state w) n ≡ in_flow state n.
+      Proof.
+        intros.
+        destruct_propagation.
+        - reflexivity.
+        - unfold in_flow; cbn. rewrite -> insert_lookup_ne by assumption. reflexivity.
+      Qed.
+
+      (* Lemma propagation_ignored: forall out state w, *)
+      (*     w ∉ dom(state.(in_flow_map)) -> w ∈ (propagate_to out state w).(work). *)
+      (* Proof. *)
+      (*   intros. destruct_propagation. - contradiction. - apply base.elem_of_list_here. *)
+      (* Qed. *)
+
+      Lemma propagation_work_update: forall out state w,
+          state.(work) ⊆ (propagate_to out state w).(work).
+      Proof.
+        intros out state w n In_state_work.
+        destruct_propagation.
+        - assumption. - apply base.elem_of_list_further. assumption.
+      Qed.
+
+      Lemma propagation_preserves_undefined: forall out state w n,
+          undefined state n -> undefined (propagate_to out state w) n.
+      Proof.
+        intros out state w n [? | ?].
+        - left. apply propagation_work_update. assumption.
+        - destruct_propagation as ? ? G.
+          + right. assumption.
+          + destruct (base.decide (n = w)).
+            * subst. left. apply base.elem_of_list_here.
+            * right. intros Falsum. cbn in Falsum.
+              apply fin_map_dom.dom_insert in Falsum.
+              rewrite -> base.elem_of_union in Falsum.
+              destruct Falsum as [ ?%sets.elem_of_singleton_1 | ? ]; contradiction.
+      Qed.
+
+      Lemma propagation_preserves_succ: forall out state w n,
+          SuccCondition n state -> SuccCondition n (propagate_to out state w).
+      Proof.
+        intros out state w n SuccCond p p_Pred_n.
+        specialize (SuccCond _ p_Pred_n) as [Undefined_p|Flow_n_w].
+        - left. apply (propagation_preserves_undefined _ _ _ _ Undefined_p).
+        - unfold out_flow in *.
+          destruct (base.decide (w = p)); subst.
+          + destruct (propagation_equ out state p) as [? | ->].
+            * in_work. assumption.
+            * satisfies_equation. rewrite -> (propagation_smaller _ _ _ n). apply Flow_n_w.
+          + satisfies_equation.
+            rewrite -> (propagation_smaller _ _ _ n).
+            rewrite -> (propagation_lookup_ne _ _ w p) by assumption.
+            apply Flow_n_w.
+      Qed.
+
+      (* Lemma fold_invariant {T U: Type}: forall (f: T -> U -> T) (P: T -> Prop), *)
+      (*     (forall a b, P a -> P (f a b)) -> *)
+      (*     forall ls a, *)
+      (*       P a -> *)
+      (*       P (fold_left f ls a). *)
+      (* Proof. *)
+      (*   intros f P Inv. induction ls as [|h t]. *)
+      (*   - intros. assumption. *)
+      (*   - intros a P_a. *)
+      (*     specialize Inv with (b := h) (1 := P_a). *)
+      (*     cbn. revert Inv. generalize (f a h). *)
+      (*     apply IHt. *)
+      (* Qed. *)
+
+      (* Lemma fold_strenghtening {T U: Type} `{base.EqDecision T}: forall (f: U -> T -> U) (Q: T -> U -> Prop) (P: T -> U -> Prop), *)
+      (*     (forall t u, P t u -> Q t u) -> *)
+      (*     (forall t u, Q t u -> P t (f u t)) -> *)
+      (*     (forall t t' u, t <> t' -> Q t u -> Q t (f u t')) -> *)
+      (*     (forall t t' u, P t u -> P t (f u t')) -> *)
+      (*     forall (ls: list T) (u: U), *)
+      (*       (forall t, t ∈ ls -> Q t u) -> *)
+      (*       forall (t: T), t ∈ ls -> P t (fold_left f ls u). *)
+      (* Proof. *)
+      (*   intros f Q P Strenghtening Intro StepPre StepPost. *)
+      (*   induction ls as [| h ls IH]; intros u Base t t_In_ls. *)
+      (*   - rewrite -> list.elem_of_nil in t_In_ls. contradiction. *)
+      (*   - apply list.elem_of_cons in t_In_ls as [<- | t_In_ls]. *)
+      (*     + cbn. *)
+      (*       apply fold_invariant. *)
+      (*       * intros. apply StepPost. assumption. *)
+      (*       * apply Intro. apply Base. apply base.elem_of_list_here. *)
+      (*     + cbn. apply IH. *)
+      (*       * clear t t_In_ls. *)
+      (*         intros t t_In_ls. *)
+      (*         destruct (base.decide (t = h)); subst. *)
+      (*         -- apply Strenghtening. apply Intro. apply Base. apply base.elem_of_list_here. *)
+      (*         -- apply StepPre. *)
+      (*            ++ assumption. *)
+      (*            ++ apply Base. apply base.elem_of_list_further. assumption. *)
+      (*       * assumption. *)
+      (* Qed. *)
+
+      Lemma fold_propagation_smaller: forall ls state out,
+          (in_flow (fold_left (propagate_to out) ls state)) ⊑ (in_flow state).
+      Proof.
+        assert (forall ls state state' out,
+                   in_flow state' ⊑ in_flow state ->
+                   (in_flow (fold_left (propagate_to out) ls state')) ⊑ (in_flow state)) as Ind. {
+
+          induction ls; intros state state' out Smaller.
+          - exact Smaller.
+          - cbn. apply IHls. rewrite -> propagation_smaller. assumption.
+        }
+        intros. apply Ind. reflexivity.
+      Qed.
+
+      Add Parametric Morphism
+        (S T: Type) `{base.Equiv S} `{base.Equiv T} (f: S -> T -> S) `{Proper_f: Proper _  ((≡) ==> (≡) ==> (≡))%signature f}:
+        (@fold_left S T f) with signature (≡) ==> (≡) ==> (≡) as list_equiv_morphis.
+      Proof.
+        intros xs ys xs_Equiv_ys.
+        induction xs_Equiv_ys as [| x y xs ys ? ? IH].
+        - intros x y x_Equiv_y. cbn. assumption.
+        - intros hl hr hl_Equiv_hr.
+          cbn. apply IH.
+          apply Proper_f; assumption.
+      Qed.
+
+      Lemma fold_propagation_lookup_nin: forall ls state out n,
+          n ∉ ls -> in_flow (fold_left (propagate_to out) ls state) n ≡ in_flow state n.
+      Proof.
+        induction ls; intros state out n n_NotIn_ls.
+        - reflexivity.
+        - rewrite -> list.not_elem_of_cons in n_NotIn_ls. destruct n_NotIn_ls as [n_NotEq_a n_NotIn_ls].
+          cbn. rewrite -> IHls by assumption.
+          apply propagation_lookup_ne.
+          symmetry. assumption.
+      Qed.
+
+      Lemma fold_propagation_lookup_in: forall ls state out n,
+          n ∈ ls -> in_flow (fold_left (propagate_to out) ls state) n ≡ in_flow state n ⊓ out.
+      Proof.
+        induction ls; intros state out n n_In_ls.
+        - apply list.elem_of_nil in n_In_ls. contradiction.
+        - cbn.
+          destruct (base.decide (n ∈ ls)).
+          + rewrite -> IHls by assumption.
+            destruct (base.decide (a = n)); subst.
+            * rewrite -> propagation_lookup_eq.
+              rewrite <- (canonical_names.associativity).
+              rewrite -> (canonical_names.idempotency _ _).
+              reflexivity.
+            * rewrite -> propagation_lookup_ne by assumption. reflexivity.
+          + assert (n = a) as <-. {
+              apply list.elem_of_cons in n_In_ls as [? | ?].
+              - assumption. - contradiction.
+            }
+            rewrite -> fold_propagation_lookup_nin by assumption.
+            rewrite ->  propagation_lookup_eq.
+            reflexivity.
+      Qed.
+
+
+      Lemma fold_propagation_lookup_lower: forall ls state out n,
+          in_flow state n ⊓ out ⊑ in_flow (fold_left (propagate_to out) ls state) n.
+      Proof.
+        intros. destruct (base.decide (n ∈ ls)).
+        - rewrite -> fold_propagation_lookup_in by assumption. reflexivity.
+        - rewrite -> fold_propagation_lookup_nin by assumption. unfold "⊓". apply orders.meet_lb_l.
+      Qed.
+
+      Lemma fold_propagation_lookup_upper: forall ls state out n,
+          in_flow (fold_left (propagate_to out) ls state) n ⊑ in_flow state n.
+      Proof.
+        intros. destruct (base.decide (n ∈ ls)).
+        - rewrite -> fold_propagation_lookup_in by assumption. unfold "⊓". apply orders.meet_lb_l.
+        - rewrite -> fold_propagation_lookup_nin by assumption. reflexivity.
+      Qed.
+
+      Lemma fold_propagation: forall ls out state,
+            Forall (fun n => in_flow (fold_left (propagate_to out) ls state) n ⊑ out) ls.
+      Proof.
+        induction ls as [| h t IH]; intros out state; cbn.
+        - constructor.
+        - specialize (IH out (propagate_to out state h)).
+          constructor; [|apply IH].
+          rewrite -> (fold_propagation_smaller _ _ _ h). rewrite -> propagation_lookup_eq. unfold "⊓". apply orders.meet_lb_r.
+      Qed.
+
+      Lemma fold_propagation': forall ls out state n,
+          n ∈ ls -> in_flow (fold_left (propagate_to out) ls state) n ⊑ out.
+      Proof.
+        intros ls out state n n_In_ls.
+        pose proof (fold_propagation ls out state) as G.
+        rewrite -> Forall_forall in G. apply G.
+        rewrite <- base.elem_of_list_In. apply n_In_ls.
+      Qed.
+
+      Lemma fold_propagation_work_lower: forall ls out state,
+          state.(work) ⊆ (fold_left (propagate_to out) ls state).(work).
+      Proof.
+        induction ls; intros.
+        - reflexivity.
+        - cbn. rewrite <- IHls. apply propagation_work_update.
+      Qed.
+
+      Lemma fold_propagation_equ: forall ls out state n,
+          let result := fold_left (propagate_to out) ls state in
+          n ∈ result.(work) \/ in_flow state n ≡ in_flow result n.
+      Proof.
+        induction ls as [| h t IH]; intros out state n result.
+        - right. reflexivity.
+        - cbn in result; subst result.
+          specialize IH with (out := out) (state := (propagate_to out state h)) (n := n) as [? | <-].
+          + left. assumption.
+          + destruct (base.decide (h = n)).
+            * subst.
+              pose proof (propagation_equ out state n) as [? | <-].
+              -- subst. left. apply fold_propagation_work_lower. assumption.
+              -- right. reflexivity.
+            * right. symmetry. apply propagation_lookup_ne. assumption.
+      Qed.
+
+      Lemma fold_propagation_equ': forall ls out state n,
+          let result := fold_left (propagate_to out) ls state in
+          in_flow state n ≢ in_flow result n -> n ∈ result.(work).
+      Proof. intros. destruct (fold_propagation_equ ls out state n). - assumption. - contradiction. Qed.
+
+      Lemma fold_propagation_preserves_undefined: forall ls out state n,
+          undefined state n -> undefined (fold_left (propagate_to out) ls state) n.
+      Proof.
+        induction ls as [| h t IH]; intros out state n Undef_n.
+        - assumption.
+        - cbn. apply IH. apply propagation_preserves_undefined. assumption.
+      Qed.
+
+      Lemma undefined_strenghtening: forall flow w work n,
+          n <> w -> undefined (mkst flow (w :: work)) n -> undefined (mkst flow work) n.
+      Proof.
+        intros flow w work n n_NotEq_w [Work_n | Ignored_n].
+        - apply list.elem_of_cons in Work_n as [? | ?]; [contradiction|]. left. assumption.
+        - right. assumption.
+      Qed.
+
+      Lemma step_loop_preserves_succ: forall  state result,
+          step state = inr result ->
+          (forall n, SuccCondition n state) ->
+          forall n, SuccCondition n result.
+      Proof.
+        intros [flow work] result Def_result SuccCond n p p_Pred_n.
+        specialize (SuccCond _ _ p_Pred_n).
+        unfold step in Def_result.
+        destruct work as [?|w work];  [discriminate|injection Def_result as Def_result].
+        destruct (base.decide (p = w)) as [? | p_NEq_w]. {
+          subst.
+          rewrite -> (fold_propagation_lookup_in) by assumption.
+          unfold out_flow.
+          destruct (fold_propagation_equ (Instance.successors w) (Instance.transfer w (flow ?! w)) (mkst flow work) w).
+          - in_work. assumption.
+          - satisfies_equation. rewrite <- H2. unfold "⊓". apply orders.meet_lb_r.
+        }
+        destruct (base.decide (in_flow (mkst flow work) p ≡ in_flow result p)) as [Unchg_p | ?]; subst.
+        - destruct SuccCond as [? | ?].
+          + left.
+            apply fold_propagation_preserves_undefined.
+            apply undefined_strenghtening with (1 := p_NEq_w).
+            assumption.
+          + satisfies_equation.
+            unfold out_flow. rewrite <- Unchg_p.
+            rewrite -> (fold_propagation_lookup_upper).
+            assumption.
+        - in_work. apply fold_propagation_equ'. assumption.
+      Qed.
+
+      Lemma step_loop_smaller: forall state result,
+          step state = inr result ->
+          in_flow result ⊑ in_flow state.
+      Proof.
+        intros [flow work] result Def_result.
+        unfold step in Def_result.
+        destruct work; cbn in Def_result.
+        - discriminate.
+        - injection Def_result as <-.
+          cbn.
+          apply fold_propagation_smaller.
+      Qed.
+
+      Lemma init_invariants: forall init,
+          Conditions init (make_init_state init).
+      Proof.
+        unfold Conditions, InitCondition, SuccCondition.
+        split.
+        - reflexivity.
+        - intros n p p_Pred_n.
+          left; unfold undefined; cbn.
+          destruct (base.decide (p ∈ dom(init))).
+          + left. rewrite -> base.elem_of_elements. assumption.
+          + right. assumption.
+      Qed.
+
+      Lemma fixpoint_invariants: forall init result,
+          fixpoint init = Some result ->
+          Conditions init (mkst result []).
+      Proof.
+        intros.
+        apply Iter.iter_prop with (P := (fun s => InitCondition init s /\ forall n, SuccCondition n s)) (3 := H2).
+        - intros s Conditions_s.
+          destruct (step s) eqn:Eq.
+          + destruct s as [flow work].
+            unfold step in Eq. destruct work; [|discriminate].
+            injection Eq as <-.
+            apply Conditions_s.
+          + split.
+            * unfold InitCondition. rewrite ->  step_loop_smaller with (1 := Eq). apply Conditions_s.
+            * apply step_loop_preserves_succ with (1 := Eq). destruct Conditions_s as [_ ?]. assumption.
+        - apply init_invariants.
+      Qed.
+
+      Lemma fixpoint_solution: forall (init result: Map) (p s: N),
+          fixpoint init = Some result ->
+          p ∈ dom(init) ->
+          s ∈ (Instance.successors p) ->
+          (result ?! s) ⊑ Instance.transfer p (result ?! p).
+      Proof.
+        intros init result p s Def_result p_In_init p_Pred_s.
+        pose proof (fixpoint_invariants init result Def_result) as [InitCond SuccCond].
+        specialize (SuccCond _ _ p_Pred_s) as [[Work_p | Ignored_p] | Equ_p_s].
+        - rewrite -> list.elem_of_nil in Work_p. contradiction.
+        - admit.
+        - apply Equ_p_s.
+      Qed.
+
+        (*
+
+          fixpoint_solution: forall (init result: Map) (n s: N),
+            fixpoint init = Some result -> n ∈ dom(init) -> s ∈ (Instance.successors n) -> (result ?! s) ⊑ Instance.transfer n (result ?! n);
+          fixpoint_invariant: forall (P: N -> A -> Prop) (init result: Map),
+            fixpoint init = Some result ->
+            (forall n, P n (init ?! n)) ->
+            (forall (p n: N) (pApprox nApprox: A), P p pApprox -> P n nApprox ->
+                                              n ∈ (Instance.successors p) ->
+                                              P n (nApprox ⊓ (Instance.transfer p pApprox))) ->
+            forall (n: N), P n (result ?! n);
+         *)
+
+    End Invariants.
+
+  Definition n_invar (s:state) (n:N.t) : Prop :=
+    In n s.(wlist) \/ forall m, In m (succs n) ->
+      s.(lmap)!!m <= trans n s.(lmap)!!n.
+
+  Definition state_invar (s:state) : Prop :=
+    forall n, NM.In n inits -> n_invar s n.
+
+  Lemma prop_n_invar_pres : forall o s n n',
+    n_invar s n -> n_invar (prop_succ o s n') n.
   Proof.
-    unfold find_default; intros.
-    erewrite M.find_1. reflexivity. apply M.add_1; auto.
+    unfold n_invar. intros.
+    set (s' := prop_succ o s n'); unfold prop_succ in s'.
+    destruct (L.eq_dec _ _); [solve [apply H]|].
+    destruct H; [solve [simpl; intuition]|].
+    destruct (N.eq_dec n n'); [solve [simpl; intuition]|].
+    right. intros.
+    destruct (N.eq_dec n' m); subst s'; simpl.
+    - subst.
+      rewrite
+        -> (find_default_eq _ _ m),
+        -> (find_default_neq _ _ m n) by auto.
+      transitivity (lmap s)!!m.
+      + apply LFacts.le_meet_l.
+      + apply H. assumption.
+    - rewrite find_default_neq, find_default_neq; auto.
   Qed.
 
-  End FMapProps.
+  (* TO MOVE *)
+  Lemma fold_left_1 : forall {A B: Type} (P:A -> Prop) (f:A -> B -> A) (bs : list B)
+                         (Hpres : forall a b, In b bs -> P a -> P (f a b)),
+      forall a a',
+        a' = fold_left f bs a -> P a -> P a'.
+  Proof.
+    intros. subst a'. generalize dependent a.
+    induction bs; simpl; intros. assumption.
+    apply IHbs. intros. apply Hpres. right; auto. assumption.
+    apply Hpres. left; auto. assumption.
+  Qed.
 
-End FMapProps.
+  (* TO MOVE *)
+  Lemma fold_left_2 : forall {A B: Type} (P:A -> B -> Prop)
+                        (f:A -> B -> A)
+                        (Hpres : forall a b b', P a b -> P (f a b') b)
+                        (Hintr : forall a b, P (f a b) b),
+      forall a a' bs b,
+        a' = fold_left f bs a ->
+        In b bs -> P a' b.
+  Proof.
+    intros. subst a'. generalize dependent a.
+    induction bs as [|b']. contradiction.
+    simpl; intros. destruct H0. subst b'.
+    set (a' := fold_left _ _ _). pattern a'.
+    eapply fold_left_1; eauto.
+    subst; reflexivity.
+    apply IHbs; assumption.
+  Qed.
 
-Module Type FORWARD_SOLVER.
+  Lemma prop_n_out : forall o ns s s' n,
+    s' = fold_left (prop_succ o) ns s ->
+    ~ In n (wlist s') ->
+    trans n (lmap s')!!n == trans n (lmap s)!!n.
+  Proof.
+    intros o ns s s' n Heqs'. pattern s'.
+    eapply fold_left_1; eauto.
+    intros. set (r := prop_succ o a b) in *.
+    unfold prop_succ in r. destruct (L.eq_dec _ _). apply H0; auto.
+    destruct (N.eq_dec b n). contradict H1; simpl; auto.
+      subst r. simpl in *. rewrite find_default_neq; auto.
+   intro. reflexivity.
+  Qed.
 
-  Declare Module L : Lattice.SemiLattice.             (* domain of approximations *)
-  Declare Module N : UsualDecidableType.  (* program points *)
+  Lemma step_state_invar : forall s s',
+    state_invar s -> inr s' = step s -> state_invar s'.
+  Proof.
+    unfold step, state_invar; intros s s' Hinv Hstep.
+    destruct (wlist s) eqn:Hwls. discriminate Hstep.
+    injection Hstep; clear Hstep. intros Heqs' n.
 
-  Declare Module NM : FMapInterface.WSfun N.
-  Module FMP := FMapProps N NM.
+    destruct (N.eq_dec t n).
 
-  (* TODO: should it really always be top?!? *)
-  Import (notations) L.
-  Notation "a !! b" := (FMP.find_default _ a b L.top)
-                         (at level 1, format "a !! b").
-  Notation nlmap := (NM.t L.t).
+    (* n_invar is restablished for n *)
+    - subst t. unfold n_invar.
+      destruct(in_dec N.eq_dec n (wlist s')) as [|Hwl]; [auto | right].
+      intros m Hin. rewrite prop_n_out; eauto; simpl.
+      generalize Hwl; clear Hwl. pattern s', m.
 
-  Parameter fixpoint: forall
-    (succs: N.t -> list N.t)
-    (trans: N.t -> L.t -> L.t)
-    (inits: nlmap),
-    option nlmap.
+      eapply fold_left_2; eauto.
+      + intros a b b'.
+        set (r := prop_succ _ a b').
+        intros. unfold prop_succ in r. destruct (L.eq_dec _ _). apply H0; auto.
+        unfold r. simpl. destruct (N.eq_dec b' b).
+        * rewrite find_default_eq; auto. apply LFacts.le_meet_r.
+        * rewrite find_default_neq; auto. apply H0. contradict Hwl; simpl; auto.
 
-  Axiom fixpoint_solution : forall
-      (succs: N.t -> list N.t)
-      (trans: N.t -> L.t -> L.t)
-      (inits: nlmap) res (n: N.t) (s: N.t),
-    fixpoint succs trans inits = Some res ->
+      + intros a b.
+        set (r := prop_succ _ a b).
+        intros. unfold prop_succ in r. destruct (L.eq_dec _ _) as [Heq|].
+        * subst r. rewrite Heq. apply LFacts.le_meet_r.
+        * simpl. rewrite find_default_eq; auto. apply LFacts.le_meet_r.
+    - (* n_invar is preserved for all successors ~= n *)
+      intros Hin. pattern s'. eapply fold_left_1; eauto.
+      intros. apply prop_n_invar_pres. assumption.
+      unfold state_invar, n_invar in Hinv |- *.
+      simpl. specialize (Hinv n). rewrite Hwls in Hinv. destruct Hinv.
+      assumption. left. destruct H; intuition. right. apply H.
+  Qed.
+
+  Lemma fixpoint_solution: forall res n s,
+    fixpoint = Some res ->
     NM.In n inits ->
     In s (succs n) ->
     res!!s <= trans n res!!n.
+  Proof.
+    unfold fixpoint; intros. pattern res.
+    eapply Iter.iter_prop with
+      (step:=step) (P:=state_invar) (a:=make_init_state); eauto.
+    - intros a Ha.
+    unfold step. destruct (wlist a) eqn:Heql.
+      + specialize (Ha n). destruct Ha.
+        * auto.
+        * rewrite Heql in *. contradiction.
+        * auto.
+      + eapply step_state_invar. apply Ha.
+        unfold step. rewrite Heql. auto.
+    - left. simpl. apply in_map_iff.
+      pose proof (NMFacts.elements_in_iff inits n0) as [He _].
+      specialize (He H2). destruct He as [e Hine].
+      apply InA_alt in Hine as [y [Heq Hk]].
+      inversion Heq; eauto.
+  Qed.
 
-  Axiom fixpoint_entry : forall succs trans inits res n,
-    fixpoint succs trans inits = Some res ->
-    res!!n <= inits!!n.
+  (* monotonicity *)
 
-  Axiom fixpoint_invariant : forall succs trans inits
+  Definition le_nlmap (nl1 nl2: nlmap) : Prop :=
+    forall n, nl1!!n <= nl2!!n.
+
+  Lemma le_nlmap_refl : forall nl, le_nlmap nl nl.
+  Proof.
+    unfold le_nlmap. reflexivity.
+  Qed.
+
+  Instance le_nlmap_trans : Transitive le_nlmap.
+    unfold Transitive, le_nlmap; intros. transitivity y !! n; auto.
+  Qed.
+
+  Hint Resolve LFacts.le_meet_l LFacts.le_meet_r : core .
+    (* L.eq_equiv L.le_preorder L.le_poset L.eq_le_reflexive. *)
+    (* Saw this in Relation_Definitions but it doesn't appear to work? *)
+
+  Lemma prop_succ_le_nlmap: forall st out n,
+    le_nlmap (prop_succ out st n).(lmap) st.(lmap).
+  Proof.
+    unfold le_nlmap, prop_succ; intros.
+    destruct (L.eq_dec _ _). reflexivity.
+    simpl. destruct (N.eq_dec n n0).
+      subst. rewrite find_default_eq; auto.
+      rewrite find_default_neq; auto. reflexivity.
+  Qed.
+
+  Lemma step_le_nlmap: forall st st',
+    inr st' = step st ->
+    le_nlmap st'.(lmap) st.(lmap).
+  Proof.
+    unfold step; intros. destruct (wlist st).
+    discriminate. injection H. intro Heqs.
+    pattern st'. eapply fold_left_1.
+    intros. transitivity (lmap a).
+       apply prop_succ_le_nlmap. assumption.
+    apply Heqs. apply le_nlmap_refl.
+  Qed.
+
+  Lemma fixpoint_entry : forall res n,
+    fixpoint = Some res -> res!!n <= inits!!n.
+  Proof.
+    unfold fixpoint. intros. pattern res.
+    eapply Iter.iter_prop with (step:=step).
+    - intros.
+      destruct (step a) eqn:Hstep.
+      + unfold step in Hstep. destruct (wlist a); try discriminate.
+        injection Hstep. intro; subst t. apply H0.
+      + simpl in *. transitivity (lmap a)!!n; [|assumption].
+        apply step_le_nlmap. auto.
+    - change inits with (lmap make_init_state).
+      cbv beta. reflexivity.
+    - apply H.
+  Qed.
+
+  Lemma fixpoint_invariant : forall
     (P: N.t -> L.t -> Prop)
     (Pinits: forall n, P n inits!!n)
     (Ptrans: forall n ln s ls,
       In s (succs n) ->
       P n ln -> P s ls -> P s (L.meet ls (trans n ln))),
-    forall res n, fixpoint succs trans inits = Some res -> P n res!!n.
+    forall res n, fixpoint = Some res -> P n res!!n.
+  Proof.
+    intros until 2.
+    unfold fixpoint. intros. pattern res.
+    eapply Iter.iter_prop with (step:=step); eauto.
 
-End FORWARD_SOLVER.
+    intro. destruct (step a) eqn:Hstep.
+
+    (* last step  Q implies P *)
+    unfold step in Hstep. destruct (wlist a); try discriminate.
+    instantiate (1:=fun s => forall n, P n s.(lmap)!!n).
+    injection Hstep. intro; subst t. intros; auto.
+
+    (* P preserved across step *)
+    simpl. intros. unfold step in Hstep.
+    destruct (wlist a); try discriminate.
+    injection Hstep; clear Hstep; intro Heqs.
+
+    pattern s. eapply fold_left_1 with (f:=prop_succ _); eauto.
+    intros. unfold prop_succ.
+    destruct (L.eq_dec _ _); simpl; auto.
+    destruct (N.eq_dec b n0).
+    rewrite find_default_eq; auto.
+      subst b. apply Ptrans; auto.
+    rewrite find_default_neq; auto.
+    auto.
+  Qed.
+
+
+    #[refine]
+    Instance solver : Solver.Analysis := {
+
+      }.
+
+
+
+  End Global.
+End Kildall.
 
 Module ForwardSolver (PC:UsualDecidableType) (LAT: Lattice.SemiLattice) <:
                      FORWARD_SOLVER with Module L := LAT
