src/coq/Analysis/Lattice.v
@@ -1,165 +1,90 @@
 Require Import List Equalities Orders RelationClasses Lia.
 Require Import FSets.
 
-(* (Bounded) (join) semi-lattice *)
+From MathClasses Require interfaces.abstract_algebra interfaces.orders orders.lattices.
+Import (hints) interfaces.abstract_algebra interfaces.orders.
+From MathClasses Require Import  interfaces.canonical_names.
+Local Open Scope mc_scope.
 
-Definition is_glb {T: Type} (le: T -> T -> Prop) (glb x y: T) :=
-  le glb x /\ le glb y /\
-    forall z, le z x -> le z y -> le z glb.
+Module Lattices.
 
-Module Type EqType.
-  Parameter t: Type.
-  Parameter eq: t -> t -> Prop.
-  #[global] Declare Instance eq_equiv : Equivalence eq.
-End EqType.
+  Module Pointwise.
+    (* Marker class enabling the pointwise lattice. *)
+    Class Pointwise (T L: Type) `{Lattice_L: @orders.LatticeOrder L Equiv_L Le_L Meet_L Join_L} := {}.
 
-(* Module Type order_SemiLattice (Import Eq: EqType). *)
-(*   (* Signature *) *)
-(*   (* Parameter t: Type. *) *)
-(*   Parameter Inline bot : t. *)
+    (* We want these instances to depent artifially on Pointwise T L, so Context cannot be used. *)
+    Instance meet `{Pointwise T L}: Meet (T -> L) := fun l r => (fun x => l x ⊓ r x).
+    Instance join `{Pointwise T L}: Join (T -> L) := fun l r => (fun x => l x ⊔ r x).
+    Instance equiv `{Pointwise T L}: Equiv (T -> L) := fun l r => ∀ x, l x = r x.
+    Instance le `{Pointwise T L}: Le (T -> L) := fun l r => forall x, l x ≤ r x.
 
-(*   (* Parameter eq: t -> t -> Prop. *) *)
-(*   Parameter le: t -> t -> Prop. *)
-  
-(*   (* (Local) notations *) *)
-(*   Infix "==" := eq (at level 70, no associativity). *)
-(*   Infix "<=" := le (at level 70, no associativity). *)
-(*   Notation "⊥" := bot (at level 0). *)
-  
-(*   (* Characterisation *) *)
-(*   (* #[global] Declare Instance eq_equiv : Equivalence eq. *) *)
-(*   #[global] Declare Instance le_preorder : PreOrder le. *)
-(*   #[global] Declare Instance le_poset : PartialOrder eq le. *)
+    Section Lattice.
+       Context `{@Pointwise T L Equiv_L Le_L Meet_L Join_L Lattice_L}.
 
-(*   Axiom ord_bot: forall x, ⊥ <= x. *)
-(*   Axiom ord_glbExists: forall x y, exists glb, is_glb le glb x y. *)
-(* End order_SemiLattice. *)
+       (* Some notations for the underlying lattice. *)
+       Infix "=ₗ" := (Equiv_L) (at level 70).
+       Infix "≤ₗ" := (Le_L) (at level 70).
+       Infix "⊓ₗ" := (Meet_L) (at level 50).
+       Infix "⊔ₗ" := (Join_L) (at level 50).
 
-(* Module Type algebraic_SemiLattice (Import Eq: EqType). *)
-(*   (* Signature *) *)
-(*   (* Parameter t: Type. *) *)
-(*   Parameter Inline bot : t. *)
-(*   Parameter join : t -> t -> t. *)
+       (* A's setoid instance is not registered as a subclass. *)
+       Local Instance setoid_L: abstract_algebra.Setoid L.
+       Proof. apply orders.po_setoid. Qed.
 
-(*   (* Parameter eq: t -> t -> Prop. *) *)
-  
-(*   (* (Local) notations *) *)
-(*   Infix "==" := eq (at level 70, no associativity). *)
-(*   Infix "∧" := join (at level 50, left associativity). *)
-(*   Notation "⊥" := bot (at level 0). *)
-  
-(*   (* Characterisation *) *)
-(*   (* #[global] Declare Instance eq_equiv : Equivalence eq. *) *)
-  
-(*   Axiom alg_botRight : forall x, x ∧ ⊥ == x. *)
-(*   Axiom alg_assoc: forall x y z, (x ∧ y) ∧ z == x ∧ (y ∧ z). *)
-(*   Axiom alg_comm: forall x y, x ∧ y == y ∧ x. *)
-(*   Axiom alg_idem: forall x, x ∧ x == x. *)
-(* End algebraic_SemiLattice. *)
+       (* Most of the following proofs will follow from the same mechanical steps:
+       - Unfold the definitions down to the lattice operations on L;
+       - Specialize all assumptions (e.g. f ≤ g) on the specific input under consideration (f x ≤ g x).
+        *)
 
-Module Type SemiLattice.
-  (* Signature *)
-  Parameter t: Type.
-  Parameter top : t.
-  Parameter meet : t -> t -> t.
+       Ltac simplifier :=
+         repeat (
+             intros ?
+             || constructor
+             || (unfold "=", "≤", "⊓", "⊔", meet, join in * )
+             || (lazymatch goal with
+                | [H: equiv _ _, x: T |- _] => specialize (H x)
+                | [H: le _ _, x: T |- _] => specialize (H x)
+                | [|- _ <-> _] => split
+                end)).
 
-  Parameter eq: t -> t -> Prop.
-  Parameter le: t -> t -> Prop.
+       (* By no means complete. *)
+       Ltac solver := try solve [
+                          repeat (
+                              lazymatch goal with
+                              | [|- ?x =ₗ ?x] => reflexivity
+                              | [|- ?x ≤ₗ ?x] => reflexivity
+                              | [H: ?T |- ?T] => exact H
+                              | [H: _ =ₗ  _ |- _] => (rewrite -> H + rewrite <- H); clear H
+                              | [H:  _ ≤ₗ _ |- _] => (rewrite -> H + rewrite <- H); clear H
+                              end)].
 
-  Parameter eq_dec: forall (l r: t), {eq l r} + {~eq l r}.
-  
-  (* Notations *)
-  Infix "==" := eq (at level 70, no associativity).
-  Infix "<=" := le (at level 70, no associativity).
-  Infix "∧" := meet (at level 50, left associativity).
-  Notation "⊤" := top (at level 0).
+       Lemma po: orders.PartialOrder le.
+       Proof.
+         simplifier; solver.
+         - (* Only antisymmetry is left. *)
+           apply antisymmetry with (R := Le_L).
+           + eauto with typeclass_instances.
+           + assumption.
+           + assumption.
+       Qed.
 
-  (* Algebraic characterisation *)
-  Axiom alg_eqCompatLeft: forall x x' y, x == x' -> x ∧ y == x' ∧ y.
-  Axiom alg_eqCompatRight: forall x y y', y == y' -> x ∧ y == x ∧ y'.
-  
-  Axiom alg_topRight : forall x, x ∧ ⊤ == x.
-  Axiom alg_assoc: forall x y z, (x ∧ y) ∧ z == x ∧ (y ∧ z).
-  Axiom alg_comm: forall x y, x ∧ y == y ∧ x.
-  Axiom alg_idem: forall x, x ∧ x == x.
+       #[export]
+       Instance mapped_lattice: orders.LatticeOrder le.
+       Proof.
+         constructor; constructor; try exact po.
+         - simplifier. apply orders.meet_lb_l.
+         - simplifier. apply orders.meet_lb_r.
+         - simplifier. apply orders.meet_glb; assumption.
+         - simplifier. apply orders.join_ub_l.
+         - simplifier. apply orders.join_ub_r.
+         - simplifier. apply orders.join_lub; assumption.
+       Qed.
 
-  (* Order-theoretic characterisation *)
-  #[global] Declare Instance eq_equiv : Equivalence eq.
-  #[global] Declare Instance le_preorder : PreOrder le.
-  #[global] Declare Instance le_poset : PartialOrder eq le.
+    End Lattice.
+  End Pointwise.
+  Export Pointwise(Pointwise).
 
-  Axiom ord_top: forall x, x <= ⊤.
-  Axiom ord_glbExists: forall x y, exists glb, is_glb le glb x y.
-
-  (* Compatibility of characterisations *)
-  Axiom characterisations_compat: forall x y, x <= y <-> x == x ∧ y.
-End SemiLattice.
-
-Module SemiLatticeFacts (Import SL: SemiLattice).
-
-  (* Relations & morphisms *)
-  (* Add Relation t eq *)
-  (*     reflexivity proved by Equivalence_Reflexive *)
-  (*     symmetry proved by Equivalence_Symmetric *)
-  (*     transitivity proved by Equivalence_Transitive *)
-  (*     as sl_eq_rel. *)
-  (* Add Relation t le *)
-  (*     reflexivity proved by PreOrder_Reflexive *)
-  (*     transitivity proved by PreOrder_Transitive *)
-  (*     as sl_le_rel. *)
-
-  Add Morphism meet with signature @eq ==> @eq ==> @eq as meet_morphism.
-  Proof.
-    intros x x' Eq_x_x' y y' Eq_y_y'.
-    apply alg_eqCompatLeft with (y := y) in Eq_x_x' as ->.
-    apply alg_eqCompatRight with (x := x') in Eq_y_y' as <-.
-    reflexivity.
-  Qed.
-
-  (* Add Morphism le with signature @eq ==> @eq ==> iff as le_morphism. *)
-  (* Proof. *)
-  (*   intros x x' Eq_x_x' y y' Eq_y_y'. *)
-  (*   rewrite -> Eq_x_x', -> Eq_y_y'.  *)
-  (*   split; intros; assumption. *)
-  (* Qed. *)
-  
-  Lemma meet_le: forall x x' y y', x <= x' -> y <= y' -> x ∧ y <= x' ∧ y'.
-  Proof.
-    intros x x' y y' Le_x_x' Le_y_y'.
-    rewrite -> characterisations_compat in *.
-    rewrite -> (alg_assoc x y _), <- (alg_assoc y x' y') , -> (alg_comm y x'), -> (alg_assoc x' y y'), <- (alg_assoc x x' _).
-    rewrite <- Le_x_x', <- Le_y_y'.
-    reflexivity.
-  Qed.
-
-  Lemma glb_uniqueness: forall x y glb glb', is_glb le glb x y -> is_glb le glb' x y -> glb == glb'.
-  Proof.
-    unfold is_glb. intros x y glb glb' (Le_glb_x & Le_glb_y & is_glb_glb) (Le_glb'_x & Le_glb'_y & is_glb_glb').
-    specialize (is_glb_glb glb' ltac:(assumption) ltac:(assumption)).
-    specialize (is_glb_glb' glb ltac:(assumption) ltac:(assumption)).
-    apply antisymmetry; assumption.
-  Qed.
-  
-  Lemma meet_is_glb: forall x y, is_glb le (x ∧ y) x y.
-  Proof.
-    intros x y. unfold is_glb.
-    split; [| split].
-    - rewrite -> characterisations_compat. rewrite -> (alg_comm x y). rewrite -> alg_assoc. rewrite -> alg_idem. reflexivity.
-    - rewrite -> characterisations_compat. rewrite -> alg_assoc. rewrite -> alg_idem. reflexivity.
-    - intros z Le_z_x Le_z_y. rewrite <- (alg_idem z). apply meet_le; assumption.
-  Qed.
-  
-  Lemma le_meet_l : forall x y, x ∧ y <= x.
-  Proof. intros. rewrite -> characterisations_compat. rewrite (alg_comm x y). rewrite -> (alg_assoc). rewrite -> (alg_idem). reflexivity. Qed.
-  
-  Lemma le_meet_r : forall x y, x ∧ y <= y.
-  Proof. intros. rewrite -> (alg_comm). apply le_meet_l. Qed.
-
-End SemiLatticeFacts.
-(* TODO: split into alg_SL and order_SL *)
-(* TODO: define lattice + injections (2) into semi lattices *)
-
-(* BoundedSets: sets with a special value representing the entire universe.
+  (* BoundedSets: sets with a special value representing the entire universe.
    - Bot: The empty set;
    - Top: The universal set;
    - Meet: Set intersection;
@@ -168,219 +93,181 @@ End SemiLatticeFacts.
 
    Note that the "bounded" in the name refers to the fact that the lattice is bounded,
    not to a bound on the size of the sets (they can be arbitratily large).
- *)
-Module BoundedSet (Import S: FSetInterface.WS) <: SemiLattice.
-  Module Import SFacts := FSetFacts.WFacts S.
-  
-  (* Set signature. *)
-  Definition t: Type := option S.t.
-  Definition empty: t := Some S.empty.
-  Definition universe: t := None.
+   *)
+  Module BoundedSet (Import S: FSetInterface.WS).
+    Module Import SFacts := FSetFacts.WFacts S.
 
-  Definition intersection (t1 t2: t): t :=
-    match t1, t2 with
+    (* Set signature. *)
+    Definition t: Type := option S.t.
+    Definition empty: t := Some S.empty.
+    Definition universe: t := None.
+
+    Definition intersection (t1 t2: t): t :=
+      match t1, t2 with
       | Some s1, Some s2 => Some (S.inter s1 s2)
       | None, Some s | Some s, None => Some s
       | None, None => None
-    end.
+      end.
 
-  Definition union (t1 t2: t) : t :=
-    match t1, t2 with
+    Definition union (t1 t2: t) : t :=
+      match t1, t2 with
       | Some s1, Some s2 => Some (S.union s1 s2)
       | None, _ | _, None => None
-    end.
+      end.
 
-  Definition singleton (e:S.elt) : t := Some (S.singleton e).
+    Definition singleton (e:S.elt) : t := Some (S.singleton e).
 
-  Definition Equal (t1 t2: t) : Prop :=
-    match t1, t2 with
+    Definition Equal (t1 t2: t) : Prop :=
+      match t1, t2 with
       | Some s1, Some s2 => s1 [=] s2
       | None, None => True
       | _, _ => False
-    end.
+      end.
 
-  Definition Subset (t1 t2: t) : Prop :=
-    match t1, t2 with
+    Definition Subset (t1 t2: t) : Prop :=
+      match t1, t2 with
       | Some s1, Some s2 => s1 [<=] s2
       | _, None => True
       | _, _ => False
-    end.
+      end.
 
-  Definition In (e:S.elt) (t:t) : Prop :=
-    match t with
+    Definition In (e:S.elt) (t:t) : Prop :=
+      match t with
       | Some s => S.In e s
       | None => True
-    end.
+      end.
 
-  (* Some props *)
-  Lemma empty_iff: forall v, In v empty <-> False.
-  Proof. intros v. cbn. apply SFacts.empty_iff. Qed.
+    Definition eq_dec : forall (x y: t), {Equal x y} + {~Equal x y}.
+      refine (fun t1 t2 => match t1, t2 with
+                        | Some s1, Some s2 => _
+                        | None, None => left _
+                        | _, _ => right _
+                        end).
+      - apply S.eq_dec.
+      - intros [].
+      - intros [].
+      - constructor.
+    Defined.
 
-  Lemma singleton_iff: forall v v', In v (singleton v') <-> S.E.eq v' v.
-  Proof. cbn. intros. apply SFacts.singleton_iff. Qed.
+    (* Some props *)
+    (* Lemma empty_iff: forall v, In v empty <-> False. *)
+    (* Proof. intros v. cbn. apply SFacts.empty_iff. Qed. *)
 
-  Lemma Equal_refl: forall t, Equal t t.
-  Proof. intros []; cbn. - reflexivity. - constructor. Qed.
+    (* Lemma singleton_iff: forall v v', In v (singleton v') <-> S.E.eq v' v. *)
+    (* Proof. cbn. intros. apply SFacts.singleton_iff. Qed. *)
 
-  Lemma Equal_symm: forall t t', Equal t t' -> Equal t' t.
-  Proof. intros [] []; cbn; firstorder. Qed.
+    (* Lemma Equal_refl: forall t, Equal t t. *)
+    (* Proof. intros []; cbn. - reflexivity. - constructor. Qed. *)
 
-  Lemma Equal_trans: forall t0 t1 t2, Equal t0 t1 -> Equal t1 t2 -> Equal t0 t2.
-  Proof. intros [] [] []; firstorder. Qed.
+    (* Lemma Equal_symm: forall t t', Equal t t' -> Equal t' t. *)
+    (* Proof. intros [] []; cbn; firstorder. Qed. *)
 
-  Lemma Subset_spec: forall a s s', In a s -> Subset s s' -> In a s'.
-  Proof. intros a s s' H H'. destruct s, s'; [|trivial|contradiction|trivial]. apply H'. apply H. Qed.
+    (* Lemma Equal_trans: forall t0 t1 t2, Equal t0 t1 -> Equal t1 t2 -> Equal t0 t2. *)
+    (* Proof. intros [] [] []; firstorder. Qed. *)
 
-  Lemma Subset_refl: forall s, Subset s s.
-  Proof. intros []; cbn; firstorder. Qed.
+    (* Lemma Subset_spec: forall a s s', In a s -> Subset s s' -> In a s'. *)
+    (* Proof. intros a s s' H H'. destruct s, s'; [|trivial|contradiction|trivial]. apply H'. apply H. Qed. *)
 
-  Lemma Subset_trans: forall s0 s1 s2, Subset s0 s1 -> Subset s1 s2 -> Subset s0 s2.
-  Proof. intros [] [] []; firstorder. Qed.
+    (* Lemma Subset_refl: forall s, Subset s s. *)
+    (* Proof. intros []; cbn; firstorder. Qed. *)
 
-  Lemma In_union: forall s t0 t1, In s (union t0 t1) -> In s t0 \/ In s t1.
-  Proof. intros s [] [] In; firstorder. cbn in *. apply S.union_1. assumption. Qed.
+    (* Lemma Subset_trans: forall s0 s1 s2, Subset s0 s1 -> Subset s1 s2 -> Subset s0 s2. *)
+    (* Proof. intros [] [] []; firstorder. Qed. *)
 
-  Add Relation t Equal
-      reflexivity proved by Equal_refl
-      symmetry proved by Equal_symm
-      transitivity proved by Equal_trans
-      as Equal_equiv.
+    (* Lemma In_union: forall s t0 t1, In s (union t0 t1) -> In s t0 \/ In s t1. *)
+    (* Proof. intros s [] [] In; firstorder. cbn in *. apply S.union_1. assumption. Qed. *)
 
-  Add Relation t Subset
-    reflexivity proved by Subset_refl
-    transitivity proved by Subset_trans
-      as Subset_order.
+    (* Add Relation t Equal *)
+    (*     reflexivity proved by Equal_refl *)
+    (*     symmetry proved by Equal_symm *)
+    (*     transitivity proved by Equal_trans *)
+    (*     as Equal_equiv. *)
 
-  Add Morphism In
-      with signature (S.E.eq) ==> (Equal) ==> iff as In_eq_mor.
-  Proof.
-    intros e e' Eq_e_e' t t' Eq_t_t'.
-    destruct t, t'; cbn in *; firstorder.
-    - rewrite <- Eq_t_t', <- Eq_e_e'. assumption.
-    - rewrite -> Eq_t_t', -> Eq_e_e'. assumption.
-  Qed.
+    (* Add Relation t Subset *)
+    (*   reflexivity proved by Subset_refl *)
+    (*   transitivity proved by Subset_trans *)
+    (*     as Subset_order. *)
 
-  Add Morphism Subset
-      with signature Equal ==> Equal ==> iff as Subset_eq_mor.
-  Proof. intros [] [] Eq0 [] [] Eq1; firstorder. Qed.
+    (* Add Morphism In *)
+    (*     with signature (S.E.eq) ==> (Equal) ==> iff as In_eq_mor. *)
+    (* Proof. *)
+    (*   intros e e' Eq_e_e' t t' Eq_t_t'. *)
+    (*   destruct t, t'; cbn in *; firstorder. *)
+    (*   - rewrite <- Eq_t_t', <- Eq_e_e'. assumption. *)
+    (*   - rewrite -> Eq_t_t', -> Eq_e_e'. assumption. *)
+    (* Qed. *)
 
-  Add Morphism In
-      with signature S.E.eq ==> Subset ==> impl as In_Subset_mor.
-  Proof.
-    intros e e' Eq_e_e' t t' Sub_t_t'.
-    destruct t, t'; cbn in *; firstorder.
-    intros ?. apply Sub_t_t'. rewrite <- Eq_e_e'. assumption.
-  Qed.
+    (* Add Morphism Subset *)
+    (*     with signature Equal ==> Equal ==> iff as Subset_eq_mor. *)
+    (* Proof. intros [] [] Eq0 [] [] Eq1; firstorder. Qed. *)
 
-  (* Lattice signature.*)
-  Definition bot: t := empty.
-  Definition top: t := universe.
+    (* Add Morphism In *)
+    (*     with signature S.E.eq ==> Subset ==> impl as In_Subset_mor. *)
+    (* Proof. *)
+    (*   intros e e' Eq_e_e' t t' Sub_t_t'. *)
+    (*   destruct t, t'; cbn in *; firstorder. *)
+    (*   intros ?. apply Sub_t_t'. rewrite <- Eq_e_e'. assumption. *)
+    (* Qed. *)
 
-  Definition meet: t -> t -> t := intersection. 
+    (* Tactic to solve core lattice equations, e.g. x ⊓ y ≤ x  *)
+    Local Ltac core_ineq_solver :=
+      intros;
+      (* Analyse whether the set is universal or regular. *)
+      (repeat lazymatch goal with
+         | [ s: t |- _ ] => destruct s as [s|]
+         end);
+      (* Discharge to firstorder if possible universal (typically when one set is universal); reduce o/w. *)
+      (try firstorder); cbn;
+      (* Split depending on goal.  *)
+      lazymatch goal with
+      | [|- _ [<=] _] => intros ? ?
+      | [|- _ [=] _] => split; intros ? ?
+      end;
+      (* Get rid of intersection&union.  *)
+      (repeat rewrite -> ?SFacts.inter_iff, -> ?SFacts.union_iff in * );
+      (* Hope for the best. *)
+      firstorder.
 
-  Definition eq := Equal.
-  Definition le := Subset.
+    Local Lemma subset_po: @orders.PartialOrder _ Equal Subset.
+    Proof.
+      constructor.
+      * (* (t, Equal) is a setoid. *)
+        constructor.
+      + (* Equal is reflexive. *)
+        intros []; firstorder.
+      + (* Equal is symmetric. *)
+        intros [] []; firstorder.
+      + (* Equal is transitive. *)
+        intros [] [] []; firstorder.
+        * (* Subset respects Equal  *)
+          intros [] [] Eq0 [] [] Eq1; firstorder.
+        * (* (t, Subset) form a pre order. *)
+          constructor.
+      + (* Subset is reflexive. *)
+        intros []; firstorder.
+      + (* Subset is transitive *)
+        intros [] [] []; firstorder.
+        * (* Subset is antisymmetric (w.r.t. Equal). *)
+          intros [] []; firstorder.
+    Qed.
 
-  Definition eq_dec : forall x y, {eq x y} + {~eq x y}.
-    refine (fun t1 t2 => match t1, t2 with
-                           | Some s1, Some s2 => _
-                           | None, None => left _
-                           | _, _ => right _
-                         end).
-    - apply S.eq_dec.
-    - intros [].
-    - intros [].
-    - constructor.
-  Defined.
-
-
-  (* Notations *)
-  Infix "==" := eq (at level 70, no associativity).
-  Infix "<=" := le (at level 70, no associativity).
-  Infix "∧" := meet (at level 50, left associativity).
-  Notation "⊥" := bot (at level 0).
-  Notation "⊤" := top (at level 0).
-
-  (* Algebraic characterisation *)
-  Lemma alg_eqCompatLeft: forall x x' y, x == x' -> x ∧ y == x' ∧ y.
-  Proof. intros [x|] [x'|] [y|] Eq_x_x'; try easy. cbn in *. rewrite -> Eq_x_x'. reflexivity. Qed.
-    
-  Lemma alg_eqCompatRight: forall x y y', y == y' -> x ∧ y == x ∧ y'.
-  Proof. intros [x|] [y|] [y'|] Eq_y_y'; try easy. cbn in *. rewrite -> Eq_y_y'. reflexivity. Qed.
-  
-  Lemma alg_topRight: forall x, x ∧ ⊤ == x.
-  Proof. intros []; easy. Qed.
-
-  Lemma alg_botRight: forall x, x ∧ ⊥ == ⊥.
-  Proof.
-    intros []; try easy. cbn. unfold bot, empty. f_equal.
-    intros x; rewrite -> inter_iff.
-    rewrite -> SFacts.empty_iff. easy.
-  Qed.
-  
-  Lemma alg_assoc: forall x y z, (x ∧ y) ∧ z == x ∧ (y ∧ z).
-  Proof. intros [] [] []; try easy. cbn. intros x. repeat rewrite -> inter_iff. easy. Qed.
-  
-  Lemma alg_comm: forall x y, x ∧ y == y ∧ x.
-  Proof. intros [] []; try easy. cbn. intros x. repeat rewrite -> inter_iff. easy. Qed.
-  
-  Lemma alg_idem: forall x, x ∧ x == x.
-  Proof. intros []; try easy. cbn. intros x. rewrite -> inter_iff. easy. Qed.
-
-  (* Order-theoretic characterisation *)
-  #[global] Instance eq_equiv : Equivalence eq.
-  Proof.
+    Instance lattice_order: @orders.LatticeOrder _ Equal Subset intersection union.
     constructor.
-    -  intros []; cbn. + reflexivity. + constructor.
-    - intros [] []; cbn; intros; easy.
-    - intros [] [] []; cbn; intros; try easy. etransitivity; eassumption.
-  Qed.
+    - (* It is an (ordered) meet semi-lattice... *)
+      constructor.
+      + exact subset_po.
+      + core_ineq_solver.
+      + core_ineq_solver.
+      + core_ineq_solver.
+    - (* ... and an (ordered) join semi-lattice. *)
+      constructor.
+      + exact subset_po.
+      + core_ineq_solver.
+      + core_ineq_solver.
+      + core_ineq_solver.
+    Qed.
 
-  #[global] Instance le_preorder : PreOrder le.
-  Proof.
-    constructor.
-    - intros []; cbn. + reflexivity. + constructor.
-    - intros [] [] []; cbn; intros; try easy. etransitivity; eassumption.
-  Qed.
-
-  #[global] Instance le_poset : PartialOrder eq le.
-  Proof.
-    intros x y. constructor.
-    - destruct x, y; intros H; cbn in *; try easy.
-      rewrite -> H.
-      split; reflexivity.
-    - destruct x, y; intros [Le_x_y Le_y_x]; cbn in *; try easy.
-      intros x; split. + apply Le_x_y. + apply Le_y_x.
-  Qed.
-
-  (* Compatibility of characterisations *)
-  Lemma characterisations_compat: forall x y, x <= y <-> x == x ∧ y.
-  Proof.
-    intros x y; split; destruct x, y; try easy; cbn.
-    - intros H x. rewrite -> inter_iff.
-      split; [| intros [? _]; assumption].
-      intros In_x. split; [assumption|].
-      rewrite -> H in In_x. assumption.
-    - intros -> x. rewrite -> inter_iff.
-      intros [_ ?]. assumption.
-  Qed.
-
-  (* Order-theoretic characterisation (cont'd) *)
-  Lemma ord_bot: forall x, ⊥ <= x.
-  Proof. intros x. rewrite -> characterisations_compat. rewrite -> alg_comm. symmetry. apply alg_botRight. Qed.
-
-  Lemma ord_top: forall x, x <= ⊤.
-  Proof. intros x. rewrite -> characterisations_compat. symmetry. apply alg_topRight. Qed.
-  
-  Lemma ord_glbExists: forall x y, exists glb, is_glb le glb x y.
-  Proof.
-    intros x y; exists (x ∧ y).
-    (* The missing parts are actual lemmas in SemiLatticeFacts *)
-    unfold is_glb. split; [|split].
-    - admit.
-    - admit.
-    - intros z Le_z_x Le_z_y.
-      rewrite <- (alg_idem z).
-      admit.
-  Admitted.
-End BoundedSet.
+    Instance bot: Bottom t := empty.
+    Instance top: Top t := universe.
+  End BoundedSet.
+End Lattices.
